Compiles but times out

src/hw.lean
@@ -8,6 +8,8 @@ import data.equiv.list
 import data.equiv.fin
 import data.equiv.fintype
 import order.lexicographic
+import data.hash_map
+import data.nat.log
 
 def arg_list (i n : ℕ) := {v : vector (fin i) n // v.to_list.nodup}
 
@@ -28,7 +30,22 @@ def rcmd.rank {i} : rcmd i → ℕ
   | (cnot _) := 2
   | (toffoli _) := 3
   | (fredkin _) := 4
- 
+
+def rcmd4.repr : rcmd 4 → string
+  | (tog a) :=
+    "n" ++ repr a.val
+  | (cnot a) :=
+    "c" ++ repr a.to_vector.head ++ repr a.to_vector.tail.head
+  | (toffoli a) :=
+    "t" ++ repr a.to_vector.head ++ repr a.to_vector.tail.head ++ repr a.to_vector.tail.tail.head
+  | (fredkin a) :=
+    "f" ++ repr a.to_vector.head ++ repr a.to_vector.tail.head ++ repr a.to_vector.tail.tail.head
+
+instance : has_repr (rcmd 4) := {
+  repr := rcmd4.repr
+}
+
+
 @[simp] lemma rcmd.rank_tog (size : ℕ) (i : fin size) : rcmd.rank (tog i) = 1 := rfl
 @[simp] lemma rcmd.rank_cnot (size : ℕ) (i) : rcmd.rank (cnot i : rcmd size) = 2 := rfl
 @[simp] lemma rcmd.rank_toffoli (size : ℕ) (i) : rcmd.rank (toffoli i : rcmd size) = 3 := rfl
@@ -45,8 +62,8 @@ open function
 def rcmd.to_nat_list {i} (x : rcmd i) : list ℕ := x.rank :: x.args.map (λ x, x.1)
 def rcmd.le {i} (x y : rcmd i) := x.to_nat_list ≤ y.to_nat_list
 lemma rcmd.le_refl {i} (x : rcmd i) : x.le x := le_refl x.to_nat_list
-lemma rcmd.le_trans {i} (x y z : rcmd i) : x.le y → y.le z → x.le z := 
-  @le_trans _ _ x.to_nat_list y.to_nat_list z.to_nat_list 
+lemma rcmd.le_trans {i} (x y z : rcmd i) : x.le y → y.le z → x.le z :=
+  @le_trans _ _ x.to_nat_list y.to_nat_list z.to_nat_list
 lemma rcmd.to_pair_injective {i} (x y : rcmd i) : x.to_nat_list = y.to_nat_list → x = y := by {
   cases x; cases y; cases x; cases y; unfold rcmd.to_nat_list rcmd.args arg_list.to_list; simp; intros h;
     apply vector.eq; exact list.map_injective_iff.mpr fin.coe_injective h,
@@ -99,10 +116,10 @@ def rcmd.run {size : ℕ} : rcmd size → array size bool → array size bool
   | (cnot {val := ⟨[control, target], _⟩, property := _}) := λ arr,
     if arr.read control then (tog target).run arr else arr
   | (toffoli {val := ⟨[control_a, control_b, target], _⟩, property := d} ) := λ arr,
-    if (arr.read control_a) 
+    if (arr.read control_a)
       then
         let d' := by {apply list.nodup_of_nodup_cons d} in
-        (cnot ⟨⟨[control_b, target], rfl⟩, d'⟩ ).run arr 
+        (cnot ⟨⟨[control_b, target], rfl⟩, d'⟩ ).run arr
       else arr
   | (fredkin {val := ⟨[control, target_a, target_b], _⟩, property := _}) := λ arr,
     if arr.read control
@@ -111,7 +128,7 @@ def rcmd.run {size : ℕ} : rcmd size → array size bool → array size bool
   using_well_founded {rel_tac := λ _ _, `[exact ⟨_, measure_wf rcmd.rank⟩]}
 
 lemma arr_write_read_neq
-  (size : ℕ) (i : fin size) {α} (arr : array size α) {x : α} : 
+  (size : ℕ) (i : fin size) {α} (arr : array size α) {x : α} :
   (arr.write i x).read i = x := by {
     exact array.read_write arr i x
 }
@@ -160,12 +177,12 @@ lemma rcmd.run_self (size : ℕ) : ∀ (c : rcmd size) (arr), c.run (c.run arr) 
   }
   | (toffoli {val := ⟨[control, control_b, target], p⟩, property := d}) := λ arr, by {
     have : (toffoli {val := ⟨[control, control_b, target], p⟩, property := d}).run =
-      λ arr, 
-        if (arr.read control) 
+      λ arr,
+        if (arr.read control)
           then
             let d' := by {apply list.nodup_of_nodup_cons d} in
-            (cnot ⟨⟨[control_b, target], rfl⟩, d'⟩ ).run arr 
-          else arr 
+            (cnot ⟨⟨[control_b, target], rfl⟩, d'⟩ ).run arr
+          else arr
       := by unfold rcmd.run,
     simp at this,
     rw this, clear this,
@@ -183,7 +200,7 @@ lemma rcmd.run_self (size : ℕ) : ∀ (c : rcmd size) (arr), c.run (c.run arr) 
       have : (((cnot {val := ⟨[control_b, target], _⟩, property := _}).run arr).read control),
       {
         have : ∀ p₁ p₂,
-          (((cnot {val := ⟨[control_b, target], p₁⟩, property := p₂}).run arr).read control) 
+          (((cnot {val := ⟨[control_b, target], p₁⟩, property := p₂}).run arr).read control)
             = arr.read control,
         {
           intros,
@@ -209,7 +226,7 @@ lemma rcmd.run_self (size : ℕ) : ∀ (c : rcmd size) (arr), c.run (c.run arr) 
     rw nodup_3 at d,
     obtain ⟨contro_ne_target_a, control_ne_target_b, target_a_ne_target_b⟩ := d,
     unfold rcmd.run,
-    have : ((arr.write target_a (arr.read target_b)).write target_b (arr.read target_a)).read control = 
+    have : ((arr.write target_a (arr.read target_b)).write target_b (arr.read target_a)).read control =
       arr.read control,
     {
       rw array.read_write_of_ne,
@@ -284,12 +301,13 @@ lemma mem_list_out (α) [fintype α] [linear_order α] (x : α) : x ∈ list_out
   exact fintype.complete x
 }
 
-#check list.mem_bind
+lemma list.mem_bind_op {α β} {b : β} {l : list α} {f : α → list β} :
+  b ∈ (l >>= f) ↔ ∃ a ∈ l, b ∈ f a := by {
+  unfold has_bind.bind,
+  apply list.mem_bind
+}
 
-lemma list.mem_bind_op {α β} {b : β} {l : list α} {f : α → list β} : 
-  b ∈ (l >>= f) ↔ ∃ a ∈ l, b ∈ f a := sorry
-
-def mem_mk_arg_list {i n} {a : arg_list i n} : 
+def mem_mk_arg_list {i n} {a : arg_list i n} :
   a ∈ (mk_arg_list (list_out (fin i)) : list (arg_list i n)) := by {
     obtain ⟨⟨l, l_length⟩, l_nodup⟩ := a,
     revert l l_length l_nodup,
@@ -304,10 +322,30 @@ def mem_mk_arg_list {i n} {a : arg_list i n} :
     },
     {
       unfold mk_arg_list,
-      
-    }
+      simp_rw list.mem_bind_op,
+      cases l,
+      {cases l_length},
+      use l_hd,
+      split,
+      {apply mem_list_out},
+      use l_tl,
+      {
+        rw list.length_cons at *,
+        exact nat.succ.inj l_length
+      },
+      {exact list.nodup_of_nodup_cons l_nodup},
+      {
+        split,
+        apply n_ih,
+        unfold mk_arg_list._match_1,
+        rw dif_neg,
+        rw list.mem_pure,
+        congr,
+        simp at *,
+        exact l_nodup.left,
+      }
+    },
   }
-
 
 def list.sort {α} [linear_order α] : list α → list α := list.merge_sort (≤)
 def multiset.sort' {α} [linear_order α] : multiset α → list α := multiset.sort (≤)
@@ -322,7 +360,7 @@ def rcmd.elems' {i} : ℕ → list (rcmd i)
 def rcmd.elems {i} : list (rcmd i) :=
   rcmd.elems' 1 ++ rcmd.elems' 2 ++ rcmd.elems' 3 ++ rcmd.elems' 4
 
-lemma rcmd.in_elems {i} (c : rcmd i) : c ∈ (rcmd.elems : list (rcmd i)) := by {
+lemma rcmd.mem_elems {i} (c : rcmd i) : c ∈ (rcmd.elems : list (rcmd i)) := by {
   cases c; unfold rcmd.elems,
   {
     repeat {apply list.mem_append_left},
@@ -342,7 +380,109 @@ lemma rcmd.in_elems {i} (c : rcmd i) : c ∈ (rcmd.elems : list (rcmd i)) := by 
     rw list.mem_map,
     use c,
     split,
-    apply mem_list_out,
-    refl,
-  }
+    apply mem_mk_arg_list,
+    refl
+  },
+  {
+    apply list.mem_append_left,
+    apply list.mem_append_right,
+    unfold rcmd.elems',
+    rw list.map_eq_map,
+    rw list.mem_map,
+    use c,
+    split,
+    apply mem_mk_arg_list,
+    refl
+  },
+  {
+    apply list.mem_append_right,
+    unfold rcmd.elems',
+    rw list.map_eq_map,
+    rw list.mem_map,
+    use c,
+    split,
+    apply mem_mk_arg_list,
+    refl
+  },
 }
+
+instance (i : ℕ) : fintype (rcmd i) := {
+  elems := rcmd.elems.to_finset,
+  complete := λ c, by { rw list.mem_to_finset, exact rcmd.mem_elems c},
+}
+
+-- this is just a type restricted version of function.comp
+infix `∘∘`:90 := λ {i}, ((∘) : (array i bool → array i bool) → (array i bool → array i bool) → (array i bool → array i bool))
+
+def list.run {i} := list.foldl (λ a (b : rcmd i), a ∘∘ b.run) id
+
+def encode_bit_list : list bool → (ℕ → ℕ) :=
+  flip (list.foldl (λ n (b : bool), if b then bit1 n else bit0 n))
+
+def list_array : ∀ {i}, list (array i bool)
+  | 0 := [array.nil]
+  | (n+1) := do
+    arr ← (list_array : list (array n bool)),
+    value ← [tt, ff],
+    pure $ array.push_back arr value
+
+def encode_array_fun {i} : (array i bool → array i bool) → (ℕ → ℕ) :=
+  λ f, encode_bit_list $
+    do
+    arr <- list_array,
+    (f arr).read <$> list_out (fin i)
+
+def pr_hash_map (i : ℕ) (n : fin 12) : Type := hash_map ℕ (λ _, vector (rcmd i) n)
+def pr_hash_map.insert {i n} : pr_hash_map i n → vector (rcmd i) n → pr_hash_map i n
+  | h v := hash_map.insert h (encode_array_fun v.to_list.run 0) v
+
+def programs2 : pr_hash_map 4 2 :=
+  list.foldl pr_hash_map.insert (mk_hash_map (2 ^ 16)) $ do
+    (c0 : rcmd 4) <- rcmd.elems,
+    (c1 : rcmd 4) <- rcmd.elems,
+    pure ⟨[c0, c1], rfl⟩
+
+def can_go_infront1' (c : rcmd 4) : list (rcmd 4) := (λ v : vector _ 2, v.head) <$>
+  list.filter (λ v : vector _ 2, v.tail.head = c) ((λ s : Σ _ : ℕ, vector (rcmd 4) 2, s.2) <$> programs2.entries)
+
+def can_go_infront : hash_map (rcmd 4) (λ _, list (rcmd 4)) :=
+  hash_map.insert_all ((λ c, ⟨c, can_go_infront1' c⟩) <$> rcmd.elems) (mk_hash_map 64)
+
+def programs3 : pr_hash_map 4 3 :=
+  let p := programs2.entries in
+  list.foldl pr_hash_map.insert (mk_hash_map (2 ^ 16)) $ do
+    ⟨_, (p1 : vector (rcmd 4) 2)⟩ <- p,
+    ⟨_, (p2 : vector (rcmd 4) 2)⟩ <- p,
+    if p2.head = p1.tail.head
+      then pure (p1.head ::ᵥ p2)
+      else []
+
+set_option profiler true
+set_option timeout 0
+
+#eval (rcmd.elems : list (rcmd 4)).length
+
+#eval programs2.entries.length
+#eval programs3.entries.length
+
+def programs5 : pr_hash_map 4 5 :=
+  list.foldl pr_hash_map.insert (mk_hash_map (2 ^ 16)) $ do
+    ⟨_, (p2 : vector (rcmd 4) 2)⟩ <- programs2.entries,
+    ⟨_, (p3 : vector (rcmd 4) 3)⟩ <- programs3.entries,
+    pure (p2.append p3)
+
+def programs10 : pr_hash_map 4 10 :=
+  list.foldl pr_hash_map.insert (mk_hash_map (2 ^ 16)) $ do
+    ⟨_, (p2 : vector (rcmd 4) 5)⟩ <- programs5.entries,
+    ⟨_, (p3 : vector (rcmd 4) 5)⟩ <- programs5.entries,
+    pure (p2.append p3)
+
+#eval programs10.entries.length
+
+#check pr_hash_map 4 11
+
+def programs11 : pr_hash_map 4 (11 : fin 12) :=
+  list.foldl pr_hash_map.insert (mk_hash_map (2 ^ 16)) $ do
+    (c : rcmd 4) <- rcmd.elems,
+    ⟨_, (p : vector (rcmd 4) 10)⟩ <- programs10.entries,
+    pure (c ::ᵥ p)
